Started eutt iff traces proof

experiments/SmallStepExperiment.v
@@ -2,6 +2,8 @@ From ITree Require Import
      ITree
      Trace.
 
+From Paco Require Import paco.
+
 Require Import List.
 Import ListNotations.
 Open Scope list_scope.
@@ -23,6 +25,7 @@ CoFixpoint big (s:state) : itree E state :=
 (* This doesn't work if the semantics loops because there can a nontrivial trace but these derivations can't find them *)
 Inductive big_trace : state -> (trace E) -> option state -> Prop :=
 | bt_done : forall s, done s = true -> big_trace s [] (Some s)
+| bt_early : forall s, done s = false -> big_trace s [] None
 | bt_tau  : forall s s' t r, done s = false -> ss s = inl s' -> big_trace s' t r -> big_trace s t r
 | bt_vis  : forall s i e k t r,
     done s = false ->
@@ -31,14 +34,29 @@ Inductive big_trace : state -> (trace E) -> option state -> Prop :=
 
 Fixpoint big_trace_approx (n:nat) (s:state) (t:trace E) (os:option state) : Prop :=
   match n with
-  | 0 => os = None /\ t = []
+  | 0 =>
+    (done s = false /\ os = None /\ t = []) \/
+    (done s = true /\ os = Some s /\ t = [])
   | S m =>
     (done s = true /\ os = Some s /\ t = []) \/
     (done s = false /\ exists s', ss s = inl s' /\ big_trace_approx m s' t os) \/
-    (done s = false /\ exists t' i e k, ss s = inr (existT _ i (e, k))
-                 (* exists? *)
-                 /\ forall (x:i), t = ((Event e x)::t') /\ (big_trace_approx m (k x) t' os))
-end.
+    (done s = false /\ exists i e k,
+        ss s = inr (existT _ i (e, k)) /\ ((t = [] /\ os = None) \/
+                                          (exists x t', t = (Event e x) :: t' /\
+                                                   big_trace_approx m (k x) t' os)))
+        (* match t with *)
+        (* | [] => True (* i uninhabited *) *)
+        (* | (Event e' x) :: t' => big_trace_approx m (k x) t' os *)
+        (* end) *)
+        (* forall (x:i) t', (big_trace_approx m (k x) t' os) -> t = ((Event e x)::t')) *)
+  end.
+
+Lemma relate : forall s t os, big_trace s t os -> exists n, big_trace_approx n s t os.
+Admitted.
+Lemma relate' : forall n s t os, big_trace_approx n s t os -> big_trace s t os.
+Admitted.
+
+(* something like (eutt t1 t2) <-> (forall t os, is_trace t1 t os <-> is_trace t2 t os) *)
 
 Lemma done_big : forall s, done s = true -> big s = Ret s.
 Proof.
@@ -71,27 +89,85 @@ Proof.
   {
     induction H.
     - rewrite (done_big _ H). constructor.
+    - constructor.
     - rewrite (not_done_big_inl _ _ H H0). constructor. auto.
     - rewrite (not_done_big_inr _ _ _ _ H H0). constructor. auto.
   }
   {
+    remember (big s) as tree.
+    induction H.
+    -
 Admitted.
 
 Lemma semantics_coincide : forall s n t os, big_trace_approx n s t os -> is_trace (big s) t os.
 Proof.
   intros s n. revert s.
   induction n; intros.
-  - red in H. destruct H. subst. constructor.
+  - red in H. destruct H.
+    + decompose [and] H; subst. constructor.
+    + decompose [and] H; subst. rewrite (done_big _ H0). constructor.
   - remember (S n) as n'. rewrite Heqn' in H.
     simpl in H. decompose [or] H; clear H.
     + decompose [and] H0; clear H0. subst. rewrite (done_big _ H). constructor.
     + decompose [ex and] H1; clear H1. subst. rewrite (not_done_big_inl _ _ H H0).
       constructor. auto.
-    + decompose [ex and] H1; clear H1. subst. rewrite (not_done_big_inr _ _ _ _ H H2).
-      constructor. auto.
+    + decompose [ex and] H1; clear H1. subst. rewrite (not_done_big_inr _ _ _ _ H H0).
+      destruct H3. subst.  destruct H1. subst. constructor.
+      decompose [ex and] H1. subst. constructor. auto.
 Qed.
 
 Lemma reverse: forall s t os, is_trace (big s) t os ->
                          exists n, big_trace_approx n s t os.
 Proof.
+  intros. remember (big s) as tree. induction H.
+  - admit.
+  -
+Admitted.
+
+Lemma is_trace_unalltaus: forall E R (t t' : itree E R) l r n,
+    is_trace t l r ->
+    unalltaus n t t' ->
+    is_trace t' l r.
+Proof.
+  intros. revert n H0. induction H; intros.
+  - constructor.
+  - rewrite (itree_eta t') in *. destruct (observe t'); inversion H0; subst; constructor.
+  - eapply IHis_trace. apply (unalltaus_tau _ _ _ H0).
+  - inversion H0; subst; clear H0. constructor. auto.
+Qed.
+
+Lemma is_trace_unalltaus': forall E R (t t' : itree E R) l r n,
+    is_trace t' l r ->
+    unalltaus n t t' ->
+    is_trace t l r.
+Proof.
+  intros. induction H0; try constructor; auto.
+Qed.
+
+Lemma eutt_traces: forall E R (t1 t2 : itree E R),
+    eutt t1 t2 <->
+    (forall t r, is_trace t1 t r <-> is_trace t2 t r).
+Proof.
+  intros. split; intros.
+  { split; intros.
+    - induction H0.
+      + constructor.
+      + assert (t2 = Ret r) by admit. subst. constructor.
+      + apply IHis_trace. admit.
+      + assert (t2 = Vis e k) by admit. subst. constructor. assumption.
+    - admit.
+  }
+  { pcofix IH. pfold. constructor; intros.
+    - split; intros.
+      + red in H0. decompose [ex] H0; clear H0. admit.
+      + (* same *) admit.
+    - assert (forall t r, is_trace t1' t r <-> is_trace t2' t r).
+      { intros. split; intros.
+        - pose proof (is_trace_unalltaus' _ _ _ _ _ _ _ H0 UNTAUS1).
+          rewrite H in H1. eapply is_trace_unalltaus; eauto.
+        - pose proof (is_trace_unalltaus' _ _ _ _ _ _ _ H0 UNTAUS2).
+          rewrite <- H in H1. eapply is_trace_unalltaus; eauto.
+      }
+      (* rewrite (itree_eta t1'). rewrite (itree_eta t2') in *. destruct (observe t1') in *; destruct (observe t2'). *)
+      admit.
 Admitted.
